Add get_insertList result to internal hashmap

src/Std/Data/DHashMap/Internal/List/Associative.lean
@@ -16,6 +16,48 @@ the contents of this file.
 File contents: Verification of associative lists
 -/
 
+-- TODO: this does not belong here; maybe create a new datatype for such dependant associative lists?
+def List.get_by_key {α : Type u} {β : α -> Type v} [BEq α] [LawfulBEq α] (l: List ((a:α) × (β a))) (k: α) (h : (l.map Sigma.fst).contains k) : β k :=
+  match l with 
+  | .nil => by simp at h
+  | .cons ⟨k', v⟩ l => if h' : k == k' 
+    then 
+      have : k = k' := LawfulBEq.eq_of_beq h'
+      cast (by rw [this]) v 
+    else List.get_by_key l k (by unfold List.map at h; rw [List.contains_cons] at h; rw [Bool.or_eq_true_iff] at h; cases h with | inl hl => simp at hl; rw [hl] at h'; simp at h' | inr _ => assumption)
+
+theorem List.get_by_key_append_elem {α : Type u} {β : α -> Type v} [BEq α] [LawfulBEq α] (l: List ((a:α) × (β a))) (elem: ((a:α) × (β a))) (k: α) (h : (l.map Sigma.fst).contains k) : ∀ h', (l ++ [elem]).get_by_key k h' = l.get_by_key k h := by 
+  intro h'
+  induction l with 
+  | nil => simp at h
+  | cons elem' l ih =>
+    simp [get_by_key]
+    split
+    . rfl
+    . apply ih
+
+theorem List.get_by_key_append_elem' {α : Type u} {β : α -> Type v} [BEq α] [LawfulBEq α] (l: List ((a:α) × (β a))) (elem: ((a:α) × (β a))) (k: α) (h : ¬(l.map Sigma.fst).contains k) : ∀ h', (l ++ [elem]).get_by_key k h' = cast (by simp at h'; simp at h; cases h' with 
+  | inl h' => cases h' with | intro a h' => specialize h a h'.left h'.right; simp at h 
+  | inr h' => rw [h']) elem.snd := 
+by 
+  intro h'
+  induction l with 
+  | nil => simp at h'; simp [get_by_key, h']
+  | cons elem' l ih =>
+    simp [get_by_key]
+    simp at h
+    simp at h'
+    cases h' with 
+    | inl h' => rw [h'] at h; simp at h
+    | inr h' => 
+      cases h' with 
+      | inl h' => cases h' with | intro a h' => have hr := h.right; specialize hr a h'.left h'.right; simp at hr
+      | inr h' =>
+        simp [h.left]
+        apply ih
+        simp
+        apply h.right
+
 set_option linter.missingDocs true
 set_option autoImplicit false
 
@@ -1871,7 +1913,7 @@ theorem insertList_perm_of_perm_first [BEq α] [EquivBEq α] (l1 l2 toInsert: Li
     exact h
     apply DistinctKeys.insertEntry distinct
 
-theorem insertList_containsKey [BEq α] [PartialEquivBEq α] (l toInsert : List ((a : α) × β a)) (k: α): containsKey k (List.insertList l toInsert) ↔ containsKey k l ∨ (toInsert.map Sigma.fst).contains k := by
+theorem containsKey_insertList [BEq α] [PartialEquivBEq α] (l toInsert : List ((a : α) × β a)) (k: α): containsKey k (List.insertList l toInsert) ↔ containsKey k l ∨ (toInsert.map Sigma.fst).contains k := by
   induction toInsert generalizing l with
   | nil => simp[insertList]
   | cons hd tl ih =>
@@ -1882,6 +1924,38 @@ theorem insertList_containsKey [BEq α] [PartialEquivBEq α] (l toInsert : List 
     rw [BEq.comm]
     conv => left; left; rw [or_comm]
     rw [or_assoc]
+
+theorem containsKey_of_containsKey_insertList [BEq α] [PartialEquivBEq α]
+    {l toInsert : List ((a : α) × β a)} {k : α} (h₁ : containsKey k (insertList l toInsert))
+    (h₂ : (toInsert.map Sigma.fst).contains k = false) : containsKey k l := by
+  rw [containsKey_insertList, h₂] at h₁; simp at h₁; exact h₁  
+
+theorem getValueCast_insertList [BEq α] [LawfulBEq α] 
+    {l toInsert : List ((a : α) × β a)} {k : α}
+    {h} : getValueCast k (insertList l toInsert) h =
+      if h' : (toInsert.map Sigma.fst).contains k then List.get_by_key toInsert.reverse k (by simp; simp at h'; exact h')
+      else getValueCast k l (containsKey_of_containsKey_insertList h (Bool.eq_false_iff.2 h')) := by
+  induction toInsert generalizing l with 
+  | nil => simp [insertList]
+  | cons elem toInsert ih => 
+    simp [insertList]
+    rw [ih]
+    split
+    case isTrue eq => 
+      split
+      case isTrue eq2 => rw [List.get_by_key_append_elem]
+      case isFalse eq2 => rw [List.contains_cons] at eq2; rw [eq] at eq2; simp at eq2
+    case isFalse eq => 
+      rw [getValueCast_insertEntry]
+      split
+      case isTrue eq2 => 
+        split 
+        case isTrue eq3 => rw [List.get_by_key_append_elem']; simp; simp at eq; exact eq
+        case isFalse eq3 => simp at eq3; simp at eq2; rw [eq2] at eq3; simp at eq3
+      case isFalse eq2 => 
+        split 
+        case isTrue eq3 => simp at eq3; simp at eq; cases eq3 with | inl hl => rw [hl] at eq2; simp at eq2 | inr hr => cases hr with | intro a hr => specialize eq a hr.left hr.right; simp at eq
+        case isFalse eq3 => rfl
 
 theorem insertList_perm [BEq α] [ReflBEq α] [PartialEquivBEq α] (l toInsert: List ((a : α) × β a)) (distinct_l: DistinctKeys l) (distinct_toInsert: DistinctKeys toInsert) (distinct_both: ∀ (a:α), ¬ containsKey a l ∨  ¬ containsKey a toInsert):
     Perm (insertList l toInsert) (l++toInsert) := by
